src/coq/CFG.v
@@ -24,7 +24,7 @@ Record pc :=
     }.
 
 Definition string_of_pc p : string :=
-  "@" ++ (string_of_raw_id (fn p)) ++ (* ":" ++ (string_of_raw_id (bn p)) ++ *) ":" ++ (string_of_instr_id (ins p)).
+  "@" ++ (string_of_raw_id (fn p)) ++ ":" ++ (string_of_instr_id (ins p)).
 
 
 Require Import Equalities.
@@ -59,7 +59,7 @@ Inductive cmd : Set :=
 .                    
 
 Inductive block_entry : Set :=
-| Phis (phis : list (local_id * instr)) (next:pt)
+| Phis (entry:pt) (phis : list (local_id * instr)) (next:pt)
 .
 
 (* each function definition corresponds to a control-flow graph *)
@@ -67,21 +67,82 @@ Record cfg := mkCFG
 {
   init : pt;
   code : pt -> option cmd; 
-  blks : block_id -> option instr_id;
   phis : block_id -> option block_entry;
+  glbl : list ident;   (* identifiers defined on entry to this CFG, 
+                          including globals and local function parameters *)
 }.
 
+(* When does a cfg program point define a given local_id. *)
+Definition pt_defines (p:pt) (lid:local_id) :=
+  match p with
+  | IId id => if id == lid then True else False
+  | IVoid _ => False
+  end.
 
-(* structurally well-formed CFGs 
-   - the initial pt denotes a command  
-   - fallthrough closure: each fallthrough pt maps to a command 
-   - jump closure: each label used in a terminator leads to a
-     block within the same function body.
-*)
+(* Which identifiers does an instruction use? *)
+Fixpoint value_uses (v:value) : list ident :=
+  match v with
+  | SV (VALUE_Ident _ id) => [id]
+  | SV (VALUE_Integer _ _)
+  | SV (VALUE_Float _ _ )
+  | SV (VALUE_Bool _ _)
+  | SV (VALUE_Null _)
+  | SV (VALUE_Zero_initializer _)
+  | SV (VALUE_Cstring _ _)
+  | SV (VALUE_None _)
+  | SV (VALUE_Undef _) => []
 
-Definition pt_exists (CFG : cfg) (p:pt) : Prop :=
-  exists cmd, (code CFG p) = Some cmd.
+  | SV (VALUE_Struct _ l)
+  | SV (VALUE_Packed_struct _ l)
+  | SV (VALUE_Array _ l)
+  | SV (VALUE_Vector _ l) => List.flat_map (fun x => value_uses (snd x)) l
+  | SV (OP_IBinop _ _ _ v1 v2) 
+  | SV (OP_ICmp _ _ _ v1 v2)
+  | SV (OP_FBinop _ _ _ _ v1 v2) 
+  | SV (OP_FCmp _ _ _ v1 v2) => (value_uses v1) ++ (value_uses v2)
+  | SV (OP_Conversion _ _ _ v _) => value_uses v
+  | SV (OP_GetElementPtr _ _ (_,ptr) idxs) => (value_uses ptr) ++ (List.flat_map (fun x => value_uses (snd x)) idxs)
+  | SV (OP_ExtractElement _  (_,vec) (_,idx)) => (value_uses vec) ++ (value_uses idx)
+  | SV (OP_InsertElement _ (_,vec) (_,elt) (_,idx)) => (value_uses vec) ++ (value_uses elt) ++ (value_uses idx)
+  | SV (OP_ShuffleVector _ (_, vec1) (_,vec2) (_,idxmask)) => (value_uses vec1) ++ (value_uses vec2) ++ (value_uses idxmask)
+  | SV (OP_ExtractValue _ (_,vec) _) => value_uses vec
+  | SV (OP_InsertValue _ (_,vec) (_,elt) _) => (value_uses vec) ++ (value_uses elt)
+  | SV (OP_Select _ (_,cnd) (_,v1) (_,v2)) => (value_uses cnd) ++ (value_uses v1) ++ (value_uses v2)
+  end.
 
+Definition tvalue_uses (tv:tvalue) : list ident := value_uses (snd tv).
+
+(* over-approximation: may include the same identifier more than once *)
+Definition instr_uses (i:instr) : (list ident) :=
+  match i with
+  | INSTR_Op op => value_uses op                         
+  | INSTR_Call (_, fid) args => [fid] ++ (List.flat_map tvalue_uses args)
+  | INSTR_Phi  t args => List.flat_map (fun x => value_uses (snd x)) args
+  | INSTR_Alloca t None align => []
+  | INSTR_Alloca t (Some tv) align => tvalue_uses tv
+  | INSTR_Load  volatile t ptr align => tvalue_uses ptr
+  | INSTR_Store volatile val ptr align => (tvalue_uses val) ++ (tvalue_uses ptr)
+  | INSTR_Fence 
+  | INSTR_AtomicCmpXchg
+  | INSTR_AtomicRMW
+  | INSTR_Unreachable
+  | INSTR_VAArg
+  | INSTR_LandingPad => []
+  end.
+
+Definition terminator_uses (t:terminator) : list ident :=
+  match t with
+  | TERM_Ret tv => tvalue_uses tv
+  | TERM_Ret_void => []
+  | TERM_Br tv _ _ => tvalue_uses tv
+  | TERM_Br_1  _ => []
+  | TERM_Switch  tv _ brs => (tvalue_uses tv) ++ (List.flat_map (fun x => tvalue_uses (fst x)) brs)
+  | TERM_IndirectBr tv _ => tvalue_uses tv
+  | TERM_Resume tv => tvalue_uses tv
+  | TERM_Invoke (_,fid) args _ _ => [fid] ++ (List.flat_map tvalue_uses args)
+  end.
+
+(* Which labels does a terminator mention *)
 Definition lbls (t:terminator) : list block_id :=
   match t with
   | TERM_Ret _        
@@ -94,55 +155,150 @@ Definition lbls (t:terminator) : list block_id :=
   | TERM_Invoke  _ _ l1 l2 => [l1; l2] 
   end.
 
-Definition is_phi (i:instr) : Prop :=
-  match i with
-   | INSTR_Phi _ _ => True
-   | _ => False
-  end.
+
+(* Well-formed SSA-form CFGs 
+   - the initial pt denotes a command  
+   - fallthrough closure: each fallthrough pt maps to a command 
+   - jump closure: each label used in a terminator leads to a
+     block within the same function body.
+   - every use of an identifier is dominated by the id's definition
+   - no identifier is defined multiple times
+*)
+Definition pt_exists (CFG : cfg) (p:pt) : Prop :=
+  exists cmd, (code CFG p) = Some cmd.
 
 
 (** Edge relation *)
-Inductive succ_pt (g:cfg) : pt -> pt -> Prop :=
-| succ_pt_S : forall p i q,
+Inductive edge_pt (g:cfg) : pt -> pt -> Prop :=
+| edge_pt_S : forall p i q,
     (code g) p = Some (Step i q) ->
-    succ_pt g p q
-| succ_pt_J : forall p b t l q,
+    edge_pt g p q
+| edge_pt_J : forall p b t l q xs r,
     (code g) p = Some (Jump b t) ->
     In l (lbls t) ->
-    (blks g) l = Some q ->
-    succ_pt g p q.
+    (phis g) l = Some (Phis q xs r) ->
+    edge_pt g p q.
 
-(*
-    (blks g) (fn p) l = Some (Phis ((x,ins)::tl) q) ->
-    succ_pt g p (mk_pt (fn p) (IId x))
-| succ_pt_Jnophi: forall p b t l q,
-    (code g) p = Some (Jump b t) ->
-    In l (lbls t) ->
-    (blks g) (fn p) l = Some (Phis [] q) ->
-    succ_pt g p q.
+(** *** GRAPH instance for dominance calculation *)
+(** Graph of program points *)
+
+Module PtGraph <: GRAPH.
+  Definition t := cfg.
+  Definition V := pt.
+  Definition entry g := init g.
+  Definition edge := edge_pt.
+  Definition mem := pt_exists.
+End PtGraph.
+
+Module Export Dom := Dom.Spec PtGraph.
+
+
+(** *** Definitions for Well-formed SSA programs. *)
+
+(** Most of the LLVM instructions define the uid associated
+  with their program point.  Some (like [store], [void] calls, and the [terminator]s)
+  do not. *)
+Definition def_at_pt (g:cfg) (p:pt) (lid:local_id) : Prop :=
+  pt_exists g p /\ pt_defines p lid.
+
+(** The definition of id dominates its use at point pt *)
+Inductive well_scoped_use_at_pt (g:cfg) (p:pt) : ident -> Prop :=
+| ws_global : forall id, In id (glbl g) -> pt_exists g p -> well_scoped_use_at_pt g p id
+| ws_local : forall lid p', def_at_pt g p' lid -> SDom g p' p -> well_scoped_use_at_pt g p (ID_Local lid).
+
+(** All uses of a [uid] must be strictly dominated by their definitions. *)
+Definition wf_use (g:cfg) (ids:list ident) (p:pt) : Prop :=
+  forall id, In id ids -> well_scoped_use_at_pt g p id.
+
+
+(** *** Well-formed phi nodes *)
+(**  Consider [ %x = phi [lbl1:v1, ...,lbln:vn] ].  This is well formed
+     when every predecessor block with terminator program point p' 
+     has a label associated with value v.  Moreover, if v uses an id then
+     the definition of the uid strictly dominates p'.
 *)
 
-Inductive wf_phis (CFG : cfg) (q : pt) : pt -> list (local_id * instr) -> Prop :=
-| wf_phis_nil : wf_phis CFG q q []
+Definition wf_phi_args (g:cfg) (entry:pt) (args:list (block_id * value)) :=
+  forall pred, edge_pt g pred entry ->
+          exists b t, (code g) pred = Some (Jump b t) /\
+                 exists v, In (b,v) args /\ wf_use g (value_uses v) pred.
+
+Inductive wf_phis (CFG : cfg) (entry:pt) (q : pt) : pt -> list (local_id * instr) -> Prop :=
+| wf_phis_nil : pt_exists CFG q ->
+                wf_phis CFG entry q q []
+
 | wf_phis_cons :
     forall p p' x t args rest,
     (code CFG p) = Some (Step (INSTR_Phi t args) p') ->
-    wf_phis CFG q p' rest ->
-    wf_phis CFG q p ((x, INSTR_Phi t args) :: rest) .
-            
-Definition wf_cfg (CFG : cfg) : Prop :=
-  pt_exists CFG (init CFG) 
-  /\ (forall p q i, (code CFG p) = Some (Step i q) -> pt_exists CFG q)
-  /\ (forall p bn t, (code CFG p) = Some (Jump bn t) ->
-               Forall (fun bn => exists p', exists xs, exists q,
-                             (blks CFG bn) = Some p' 
-                             /\ (phis CFG bn) = Some (Phis xs q) 
-                             /\ wf_phis CFG q p' xs
-                             /\ pt_exists CFG q
-                      )
-                      (lbls t)).
+    wf_phi_args CFG entry args ->
+    wf_phis CFG entry q p' rest ->
+    wf_phis CFG entry q p ((x, INSTR_Phi t args) :: rest) .
 
-Lemma wf_cfg_succ_pt : forall g p1 p2, wf_cfg g -> pt_exists g p1 -> succ_pt g p1 p2 -> pt_exists g p2.
+Inductive wf_cmd (g:cfg) (p:pt) : cmd -> Prop :=
+| wf_step : forall (i:instr) (q:pt)
+              (Hq : pt_exists g q)
+              (Huse: wf_use g (instr_uses i) p),
+    wf_cmd g p (Step i q)
+
+| wf_jump : forall (bn:block_id) (t:terminator)
+              (Huse: wf_use g (terminator_uses t) p)
+              (Hlbls: Forall (fun tgt => exists p', exists xs, exists q,
+                             (phis g tgt) = Some (Phis p' xs q) 
+                             /\ wf_phis g p' q p' xs
+                      )
+                      (lbls t)),
+    wf_cmd g p (Jump bn t).
+
+
+(* TODO: do we have to worry about locals shadowing function parameters? 
+   Could add: forall lid, In (ID_Local lid) (glbl CFG) -> (code CFG) (IId lid) = None
+
+   - also, somewhere probably need that globals and function parameters are distinct
+ *)
+
+Definition wf_cfg (CFG : cfg) : Prop :=
+  pt_exists CFG (init CFG)
+  /\ forall p, ~ edge_pt CFG p (init CFG)            
+  /\ (forall p cmd, (code CFG p) = Some cmd -> wf_cmd CFG p cmd)
+.
+
+(*
+  Definition wf_phi_args (g:Cfg.t) (i:insn) (p:pc) : Prop :=
+    forall pred, edge_pt g pred (entry_of_pc p) ->
+      (exists v, In (lbl_of pred, v) (insn_phis i)) /\
+      (forall uid, In (lbl_of pred, val_uid uid) (insn_phis i) -> 
+          uid_sdom_pc g uid pred).
+
+  Definition wf_phi_pred (g:Cfg.t) (i:insn) (p:pc) : Prop :=
+    forall l v, In (l, v) (insn_phis i) ->
+      (exists pred, edge_pt g pred (entry_of_pc p) /\ lbl_of pred = l).
+
+  Definition wf_phi (g:Cfg.t) (i:insn) (p:pc) : Prop :=
+    is_phi i -> wf_phi_args g i p
+             /\ wf_phi_pred g i p
+             /\ insn_phis i <> [].
+
+  (** *** Well-formed instructions *)
+
+  Inductive wf_insn (g:Cfg.t) : insn -> pc -> Prop :=
+  | wf_insn_intro : forall i p,
+      wf_use g i p ->
+      wf_lbl g i ->
+      wf_phi g i p ->
+      wf_insn g i p.
+
+  Inductive wf_prog (g:Cfg.t) : Prop :=
+  | wf_prog_intro : forall
+      (Hwfcfg : wf_cfg g)
+      (Hwfis : forall p i, insn_at_pc g p i -> wf_insn g i p)
+      (Hwftmn : forall p' i, tmn_pc g p' -> insn_at_pc g p' i -> is_tmn i)
+      (Hwfentry : forall p, ~ edge_pt g p (block_entry (entry_block g))),
+      wf_prog g.
+
+
+            
+Lemma wf_cfg_edge_pt : forall g p1 p2,
+    wf_cfg g -> pt_exists g p1 -> edge_pt g p1 p2 -> pt_exists g p2.
 Proof.
   intros g p1 p2 H H0 H1.
   destruct H as [Hinit [HStep HJump]].
@@ -158,6 +314,9 @@ Proof.
     * exists (Step (INSTR_Phi t0 args) p').
       exact H.
 Qed.      
+*)
+
+
 
 
 
@@ -173,40 +332,38 @@ Fixpoint lookup_function_definition ets f : option definition :=
       lookup_function_definition ts f
   | _ :: ts => lookup_function_definition ts f
   end.
-                                                 
-Fixpoint init_of_definition d : option pt :=
-  match (df_instrs d) with
-  | [] => None
-  | b :: _ => Some (match blk_instrs b with
-                   | [] => blk_term_id b
-                   | (iid, _) :: t => iid
-                   end)
-  end.
 
-
-Fixpoint phis_from_block term_id (b : list (instr_id * instr)) : option block_entry :=
-  match b with
-    | (IId iid, INSTR_Phi i v as ins) :: t =>
-       'rest <- phis_from_block term_id t;
-        match rest with
-          | Phis phis p => Some (Phis ((iid, ins)::phis) p) 
-        end
-    | (IVoid _, INSTR_Phi i v as ins) :: t => None
-    | (next, _) :: _ => Some (Phis [] next)
-    | [] => Some (Phis [] term_id)
-  end.
-
-Fixpoint lookup_block bs block_id : option block :=
-  find (fun b => if (blk_id b) == block_id then true else false) bs.
-
-Fixpoint block_to_phis (b:block) : option block_entry :=
-  phis_from_block (blk_term_id b) (blk_instrs b).
-  
 Definition fallthrough term_id (is : list (instr_id * instr)) : instr_id :=
   match is with
   | [] => term_id
   | (next, _)::_ => next
   end.
+
+Definition blk_entry (b:block) := fallthrough (blk_term_id b) (blk_instrs b). 
+
+Definition init_of_definition d : option pt :=
+  match (df_instrs d) with
+  | [] => None
+  | b :: _ => Some (blk_entry b)
+  end.
+
+Fixpoint phis_from_block entry term_id (b : list (instr_id * instr)) : option block_entry :=
+  match b with
+    | (IId iid, INSTR_Phi i v as ins) :: t =>
+       'rest <- phis_from_block entry term_id t;
+        match rest with
+          | Phis _ phis p => Some (Phis entry ((iid, ins)::phis) p) 
+        end
+    | (IVoid _, INSTR_Phi i v as ins) :: t => None
+    | (next, _) :: _ => Some (Phis entry [] next)
+    | [] => Some (Phis entry [] term_id)
+  end.
+
+Fixpoint block_to_phis (b:block) : option block_entry :=
+  phis_from_block (blk_entry b) (blk_term_id b) (blk_instrs b).
+  
+Fixpoint lookup_block bs block_id : option block :=
+  find (fun b => if (blk_id b) == block_id then true else false) bs.
 
 Fixpoint lookup_instr (p:pt) term_id (insns : list (instr_id * instr)) : option cmd :=
   match insns with
@@ -247,107 +404,31 @@ Definition phis_of_definition (d:definition) block_id : option block_entry :=
   'b <- lookup_block (df_instrs d) block_id;
   block_to_phis b.
 
-Definition cfg_of_definition (d:definition) : option cfg :=
+Definition cfg_of_definition (g:list ident) (d:definition) : option cfg :=
   'init <- init_of_definition d;
     Some {| init := init;
             code := code_of_definition d;
-            blks := blks_of_definition d;
-            phis := phis_of_definition d
+            phis := phis_of_definition d;
+            glbl := g;
          |}.
             
-Definition fcfg := function_id -> option (list ident * cfg).
+Definition fcfg := function_id -> option (list local_id * cfg).
 
-Fixpoint entities_to_funs ets fid : option (list ident * cfg) :=
+Definition globals_of (tle : toplevel_entity) : list ident :=
+  match tle with
+  | TLE_Declaration d => [ID_Global (dc_name d)]
+  | TLE_Definition d => [ID_Global (dc_name (df_prototype d))]
+  | TLE_Global g => [ID_Global (g_ident g)]
+  | _ => []
+  end.
+
+Definition globals (ets : list toplevel_entity) : list ident :=
+  List.fold_right (fun tle acc => (globals_of tle) ++ acc) [] ets.
+
+Fixpoint entities_to_funs ets fid : option (list local_id * cfg) :=
   'd <- lookup_function_definition ets fid;
-  'cfg <- cfg_of_definition d;
-  Some (map (fun x => ID_Local x) (df_args d), cfg).
+    let args := List.map (fun x => ID_Local x) (df_args d) in
+    let g := globals ets in
+    'cfg <- cfg_of_definition (g++args) d;
+    Some (df_args d, cfg).
 
-
-(*
-
-Module Wellformedness.
-
-
-  (** *** GRAPH instance for dominance calculation *)
-
-
-  (** Graph of program points *)
-
-  Module PcGraph <: GRAPH.
-    Definition t := cfg.
-    Definition V := pt.
-    Definition entry g := init g.
-    Definition Succ := succ_pt.
-    Definition Mem := pt_exists.
-  End PcGraph.
-
-  Module Export Dom := Dom.Spec PcGraph.
-
-  (** *** Definitions for Well-formed SSA programs. *)
-
-  (** FULL: Most of the Vminus instructions define the uid associated
-  with their program point.  Some (like [store] and the [tmn]s)
-  do not. *)
-  (** TERSE: The command at the given [pc] defines uid. *)
-
-  Definition def_at_pc (g:cfg) (p:pt) (uid:uid) : Prop :=
-    exists c, insn_at_pc g p (uid, c) /\ defs_uid (uid, c). 
-
-  (** The definition of [uid] strictly dominates the pc. *)
- 
-  Definition uid_sdom_pc (g:Cfg.t) (uid:uid) (p:pc) : Prop :=
-    exists p', def_at_pc g p' uid /\ SDom g p' p.
-
-  (** All uses of a [uid] must be strictly dominated by
-      their definitions. *)
-
-  Definition wf_use (g:Cfg.t) (i:insn) (p:pc) : Prop :=
-    forall uid, In (val_uid uid) (insn_uses i) -> uid_sdom_pc g uid p.
-
-  (** All jump targets must be legal block labels. *)
-
-  Definition wf_lbl (g:Cfg.t) (i:insn) : Prop :=
-    forall l, In l (insn_lbls i) -> wf_pc g (block_entry l).
-
-  (** *** Well-formed phi nodes *)
-
-  (**  Consider [ %x = phi [lbl1:v1, ...,lbln:vn] ].  This is well formed
-       when every predecessor block with terminator program point p' 
-       has a label associated with value v.  Moreover, if v is a uid then
-       the definition of the uid strictly dominates p'.
-  *)
-
-  Definition wf_phi_args (g:Cfg.t) (i:insn) (p:pc) : Prop :=
-    forall pred, succ_pt g pred (entry_of_pc p) ->
-      (exists v, In (lbl_of pred, v) (insn_phis i)) /\
-      (forall uid, In (lbl_of pred, val_uid uid) (insn_phis i) -> 
-          uid_sdom_pc g uid pred).
-
-  Definition wf_phi_pred (g:Cfg.t) (i:insn) (p:pc) : Prop :=
-    forall l v, In (l, v) (insn_phis i) ->
-      (exists pred, succ_pt g pred (entry_of_pc p) /\ lbl_of pred = l).
-
-  Definition wf_phi (g:Cfg.t) (i:insn) (p:pc) : Prop :=
-    is_phi i -> wf_phi_args g i p
-             /\ wf_phi_pred g i p
-             /\ insn_phis i <> [].
-
-  (** *** Well-formed instructions *)
-
-  Inductive wf_insn (g:Cfg.t) : insn -> pc -> Prop :=
-  | wf_insn_intro : forall i p,
-      wf_use g i p ->
-      wf_lbl g i ->
-      wf_phi g i p ->
-      wf_insn g i p.
-
-  Inductive wf_prog (g:Cfg.t) : Prop :=
-  | wf_prog_intro : forall
-      (Hwfcfg : wf_cfg g)
-      (Hwfis : forall p i, insn_at_pc g p i -> wf_insn g i p)
-      (Hwftmn : forall p' i, tmn_pc g p' -> insn_at_pc g p' i -> is_tmn i)
-      (Hwfentry : forall p, ~ succ_pt g p (block_entry (entry_block g))),
-      wf_prog g.
-
-End Wellformedness.
-*)
